src/Examples/ECC/CondSwap.v
@@ -1,0 +1,49 @@
+Require Import Rupicola.Lib.Api.
+
+Section Gallina.
+  Definition cswap {T} (swap:bool) (a b: T) : T * T :=
+    if swap then (b, a) else (a, b).
+End Gallina.
+
+Section Compile.
+  Context {semantics : Semantics.parameters}
+          {semantics_ok : Semantics.parameters_ok semantics}.
+
+  (* There are two ways cswap could be compiled; you can either swap the local
+     variables (the pointers), or you can leave the pointers and copy over the
+     data. This version swaps the pointers without doing any copying. *)
+  Lemma compile_cswap_nocopy :
+    forall (locals: Semantics.locals) (mem: Semantics.mem)
+      tr R R' functions T (pred: T -> _ -> Prop)
+      {data} (x y : data) swap x_var x_ptr y_var y_ptr k k_impl
+      (Data : word -> data -> Semantics.mem -> Prop) var,
+      x_var <> y_var ->
+      x_var <> var ->
+      var <> y_var ->
+      map.get locals x_var = Some x_ptr ->
+      map.get locals y_var = Some y_ptr ->
+      (Data x_ptr x * Data y_ptr y * R')%sep mem ->
+      let v := cswap swap x y in
+      (let head := v in
+       (find k_impl
+        implementing (pred (k head))
+        with-locals
+               (map.put (map.put (map.put locals var x_ptr) x_var y_ptr)
+                        y_var x_ptr)
+        and-memory mem and-trace tr and-rest R
+        and-functions functions)) ->
+      (let head := v in
+       find (cmd.seq
+               (cmd.seq
+                  (cmd.seq
+                     (cmd.set var (expr.var x_var))
+                     (cmd.set x_var (expr.var y_var)))
+                  (cmd.set y_var (expr.var var)))
+               k_impl)
+       implementing (pred (dlet head k))
+       with-locals locals and-memory mem and-trace tr and-rest R
+       and-functions functions).
+  Proof.
+    repeat straightline'. subst_lets_in_goal. eauto.
+  Qed.
+End Compile.
